
\documentclass[11pt]{article}
%%%%%%%%%%%%%%%%%%%%%%%%%%%%%%%%%%%%%%%%%%%%%%%%%%%%%%%%%%%%%%%%%%%%%%%%%%%%%%%%%%%%%%%%%%%%%%%%%%%%%%%%%%%%%%%%%%%%%%%%%%%%%%%%%%%%%%%%%%%%%%%%%%%%%%%%%%%%%%%%%%%%%%%%%%%%%%%%%%%%%%%%%%%%%%%%%%%%%%%%%%%%%%%%%%%%%%%%%%%%%%%%%%%%%%%%%%%%%%%%%%%%%%%%%%%%
\usepackage{amsmath}
\usepackage{beamerarticle}
\usepackage{fullpage}
\usepackage{pgf}
\usepackage{hyperref}
\usepackage{graphics}

\setcounter{MaxMatrixCols}{10}

\mode<article> {
}
\mode<article> {}
\oddsidemargin 0in \textwidth 6.25in
\topmargin -0in \textheight 8.25in
\begin{document}

\setlength{\baselineskip}{1.5\baselineskip}
\textbf{Note of Demand Elasticities}\\

Recall that we have the following share equations from AIDS 
\begin{eqnarray}
\omega_i = \alpha_i + \sum_{j} \gamma_{ij}lnp_j +\beta_i ln(\frac{X}{P}), \forall i \\
lnP=\alpha_0 + \sum_{j}\alpha_j lnp_j + \frac{1}{2}\sum_i\sum_j \gamma_{ij} lnp_i lnp_j
\end{eqnarray}
and if we use Stone approximation
\begin{eqnarray}
ln\tilde{P}=\sum_{k}\omega_k lnp_k
\end{eqnarray}

We first show that $\frac{d\omega_i}{dlnp_j}$ is connected to demand elasticities $\frac{dlnq_i}{dlnp_j}$.\\
If $i = j$, i.e., we are interested in own elasticity, then
\begin{eqnarray}
\frac{d\omega_i}{dlnp_j}=\frac{d(p_iq_i)}{dlnp_i}\cdot\frac{1}{X}=[p_iq_i+\frac{dq_i}{dlnp_i}p_i]/X= \frac{p_iq_i}{X}[1+\frac{dlnq_i}{dlnp_i}] \equiv \omega_i[1+\eta_{ii}]
\end{eqnarray}
where $\eta_{ii}$ is the own demand elasticity. \\
If $i\neq j$, i.e., we are interested in cross elasticity, then
\begin{eqnarray}
\frac{d\omega_i}{dlnp_j}=\frac{d(p_iq_i)}{dlnp_j}\cdot\frac{1}{X}=[0+\frac{dq_i}{dlnp_j}p_i]/X= \frac{p_iq_i}{X}\frac{dlnq_i}{dlnp_j}\equiv \omega_i\eta_{ij}
\end{eqnarray}
where $\eta_{ij}$ is the cross demand elasticity.\\
Making use of the AIDS demand system, we know that
\begin{eqnarray}
\frac{d\omega_i}{dlnp_j}=\gamma_{ij}-\beta_i \frac{dlnP}{dlnp_j}
\end{eqnarray}
Thus the bottom-line is that we have
\begin{eqnarray}
\eta_{ii} = -1 + [\gamma_{ii}-\beta_i \frac{dlnP}{dlnp_i}]/\omega_i\\
\eta_{ij} = [\gamma_{ij}-\beta_i \frac{dlnP}{dlnp_j}]/\omega_i
\end{eqnarray}
Finally, the calculation of $\frac{dlnP}{dlnp_j}$ can either use AIDS exact price aggregation
\begin{eqnarray}
\frac{dlnP}{dlnp_j} = \alpha_j +\sum_{k}\gamma_{kj} lnp_k
\end{eqnarray}
or use Stone approximation formula (by assuming a constant expenditure share)\footnote{Alston et al (94) shows this is a pretty good approximation with Monte Carlo Simulations.}
\begin{eqnarray}
\frac{dlnP}{dlnp_j} = \omega_j
\end{eqnarray}


\end{document} 